theories/language/metatheory.v
@@ -27,7 +27,6 @@ Fixpoint expr_closed X e :=
       expr_closed (set_binder_insert f (set_binder_insert x X)) e
   | Unop _ e
   | Proj _ e
-  | Constr _ e
   | Fork e
   | Load e =>
       expr_closed X e
@@ -40,13 +39,15 @@ Fixpoint expr_closed X e :=
   | Faa e1 e2 =>
       expr_closed X e1 && expr_closed X e2
   | If e0 e1 e2
-  | Case e0 e1 e2
   | Cas e0 e1 e2
   | Resolve e0 e1 e2 =>
       expr_closed X e0 && expr_closed X e1 && expr_closed X e2
   | Tuple es
+  | Constr _ es
   | Record es =>
       forallb (expr_closed X) es
+  | Case e brs =>
+      expr_closed X e && forallb (λ br, expr_closed X br.2) brs
   | Proph =>
       true
   end
@@ -58,56 +59,8 @@ with val_closed v :=
       expr_closed (set_binder_insert f (set_binder_insert x ∅)) e
   | ValTuple vs =>
       forallb val_closed vs
-  | ValConstr _ v =>
-      val_closed v
-  end.
-
-Fixpoint subst_map (vs : gmap string val) e :=
-  match e with
-  | Val _ =>
-      e
-  | Var y =>
-      if vs !! y is Some v then Val v else Var y
-  | Rec f y e =>
-      Rec f y $ subst_map (binder_delete y (binder_delete f vs)) e
-  | App e1 e2 =>
-      App (subst_map vs e1) (subst_map vs e2)
-  | Unop op e =>
-      Unop op $ subst_map vs e
-  | Binop op e1 e2 =>
-      Binop op (subst_map vs e1) (subst_map vs e2)
-  | Equal e1 e2 =>
-      Equal (subst_map vs e1) (subst_map vs e2)
-  | If e0 e1 e2 =>
-      If (subst_map vs e0) (subst_map vs e1) (subst_map vs e2)
-  | Tuple es =>
-      Tuple $ subst_map vs <$> es
-  | Proj i e =>
-      Proj i $ subst_map vs e
-  | Constr b e =>
-      Constr b $ subst_map vs e
-  | Case e0 e1 e2 =>
-      Case (subst_map vs e0) (subst_map vs e1) (subst_map vs e2)
-  | Fork e =>
-      Fork $ subst_map vs e
-  | Record es =>
-      Record $ subst_map vs <$> es
-  | Alloc e1 e2 =>
-      Alloc (subst_map vs e1) (subst_map vs e2)
-  | Load e =>
-      Load $ subst_map vs e
-  | Store e1 e2 =>
-      Store (subst_map vs e1) (subst_map vs e2)
-  | Xchg e1 e2 =>
-      Xchg (subst_map vs e1) (subst_map vs e2)
-  | Cas e0 e1 e2 =>
-      Cas (subst_map vs e0) (subst_map vs e1) (subst_map vs e2)
-  | Faa e1 e2 =>
-      Faa (subst_map vs e1) (subst_map vs e2)
-  | Proph =>
-      Proph
-  | Resolve e0 e1 e2 =>
-      Resolve (subst_map vs e0) (subst_map vs e1) (subst_map vs e2)
+  | ValConstr _ vs =>
+      forallb val_closed vs
   end.
 
 #[local] Instance set_unfold_elem_of_insert_binder x y X Q :
@@ -126,7 +79,8 @@ Proof.
     rewrite ?bool_decide_spec ?andb_True => ? ?;
     repeat case_decide; simplify_eq/=; f_equal; intuition eauto with set_solver.
   all: select (Forall _ _) ltac:(fun H => induction H; first done).
-  all: rewrite fmap_cons; f_equal; naive_solver.
+  all: try select branch ltac:(fun br => destruct br).
+  all: rewrite fmap_cons; repeat f_equal; naive_solver.
 Qed.
 
 Lemma subst_closed_empty e x v :
@@ -141,8 +95,8 @@ Lemma subst_subst e x v v' :
 Proof.
   intros. induction e; simpl; try (f_equal; auto; done);
     simplify_option_eq; auto using subst_closed_empty with f_equal.
-  all: select (Forall _ _) ltac:(fun H => induction H; first done).
-  all: rewrite !fmap_cons; do 2 f_equal; naive_solver.
+  all: select (Forall _ _) ltac:(fun H => induction H).
+  all: naive_solver congruence.
 Qed.
 Lemma subst_subst' e x v v' :
   subst' x v (subst' x v' e) = subst' x v' e.
@@ -156,8 +110,8 @@ Lemma subst_subst_ne e x y v v' :
 Proof.
   intros. induction e; simpl; try (f_equal; by auto);
     simplify_option_eq; auto using eq_sym, subst_closed_empty with f_equal.
-  all: select (Forall _ _) ltac:(fun H => induction H; first done).
-  all: rewrite !fmap_cons; do 2 f_equal; naive_solver.
+  all: select (Forall _ _) ltac:(fun H => induction H).
+  all: naive_solver congruence.
 Qed.
 Lemma subst_subst_ne' e x y v v' :
   x ≠ y →
